theories/Utils/BitVectors.v
@@ -62,10 +62,10 @@ Theorem iffb_beq : forall {b1 b2}, (iffb b1 b2 = true) <-> b1 = b2.
   intro x; discriminate x.
 Qed.
 
-Definition bv_eq {n} (b1 b2 : t bool n) : bool.
-  apply (fun x : {b1 = b2} + {b1 <> b2} => if x then true else false).
-  apply (VectorEq.eq_dec bool iffb (@iffb_beq)).
-Defined.
+Definition bv_eq {n} : t bool n -> t bool n -> bool :=
+  rect2 (fun _ _ _ => bool)
+        true
+        (fun _ xs ys r x y => andb (iffb x y) r).
 
 Definition bv_and {n} (b1 b2 : t bool n) : t bool n :=
   map2 andb b1 b2.
@@ -233,28 +233,28 @@ Definition bitvector_fin_big : forall {n},
       assumption.
 Defined.
 
-Definition bitvector_fin_big_fun {n} (v : t bool n) : nat :=
+Definition bitvector_nat_big {n} (v : t bool n) : nat :=
   proj1_sig (bitvector_fin_big v).
 
-Theorem bitvector_fin_big_fun_lt_2pow {n} (v : t bool n) :
-  bitvector_fin_big_fun v < 2 ^ n.
+Theorem bitvector_nat_big_lt_2pow {n} (v : t bool n) :
+  bitvector_nat_big v < 2 ^ n.
 Proof.
-  unfold bitvector_fin_big_fun.
+  unfold bitvector_nat_big.
   destruct (bitvector_fin_big v) as [f fP].
   assumption.
 Qed.
 
-Fixpoint fin_bitvector_big_fun (n m : nat) : t bool n :=
+Fixpoint nat_bitvector_big (n m : nat) : t bool n :=
   match n with
   | 0 => nil bool
   | S n => 
-    cons _ (negb (m / (2 ^ n) =? 0)) _ (fin_bitvector_big_fun n (m mod 2 ^ n))
+    cons _ (negb (m / (2 ^ n) =? 0)) _ (nat_bitvector_big n (m mod 2 ^ n))
   end.
 
 Definition fin_bitvector_big : forall {n},
   fin (2 ^ n) -> t bool n.
   intros n [f _].
-  apply (fin_bitvector_big_fun n f).
+  apply (nat_bitvector_big n f).
 Defined.
 
 Theorem bitvector_fin_big_cons_lem : forall {n},
@@ -278,20 +278,31 @@ Proof.
   simpl; apply subset_eq_compat; lia.
 Qed.
 
-Theorem bitvector_fin_big_fun_inv : forall {n} (v : t bool n),
-  fin_bitvector_big_fun n (bitvector_fin_big_fun v) = v.
+Theorem bitvector_nat_big_cons : forall {n} x (v : t bool n),
+  bitvector_nat_big (x :: v) =
+  proj1_sig (bitVal x) * 2^n + bitvector_nat_big v.
+Proof.
+  intros n x v.
+  unfold bitvector_nat_big at 1.
+  rewrite bitvector_fin_big_cons, proj1_fin_cast,
+          proj1_fin_add, proj1_fin_mul, proj1_fin_max.
+  reflexivity.
+Qed.
+
+Theorem bitvector_nat_big_inv : forall {n} (v : t bool n),
+  nat_bitvector_big n (bitvector_nat_big v) = v.
 Proof.
   intros n v.
-  unfold bitvector_fin_big_fun.
   induction v.
   - reflexivity.
-  - rewrite bitvector_fin_big_cons.
-    rewrite proj1_fin_cast, proj1_fin_add, proj1_fin_mul, proj1_fin_max.
-    unfold fin_bitvector_big_fun; fold fin_bitvector_big_fun.
+  - assert (bitvector_nat_big v < 2 ^ n).
+    { apply bitvector_nat_big_lt_2pow. }
+    rewrite bitvector_nat_big_cons.
+    unfold nat_bitvector_big; fold nat_bitvector_big.
     f_equal.
     + destruct (bitvector_fin_big v); destruct h; simpl proj1_sig.
       * rewrite PeanoNat.Nat.mul_1_l.
-        replace ((2 ^ n + _) / _) with 1. { reflexivity. }
+        replace (_ / _) with 1. { reflexivity. }
         symmetry; apply div_bet_1; lia.
       * rewrite PeanoNat.Nat.mul_0_l, div_small; simpl; lia.
     + assert (2 ^ n <> 0) as pow0.
@@ -300,6 +311,7 @@ Proof.
       { apply IHv. }
       rewrite <- PeanoNat.Nat.add_mod_idemp_l.
       2: { assumption. }
+      unfold bitvector_nat_big.
       replace ((proj1_sig (bitVal h) * 2 ^ n) mod 2 ^ n)
          with 0.
       destruct (bitvector_fin_big v) as [f fP].
@@ -310,19 +322,11 @@ Proof.
         apply zero2pow.
 Qed.
 
-Theorem bitvector_fin_big_lim : forall {n} (v : t bool n),
-    bitvector_fin_big_fun v < 2 ^ n.
-Proof.
-  intros n v.
-  unfold bitvector_fin_big_fun.
-  destruct (bitvector_fin_big v); trivial.
-Qed.
-
 Theorem bitvector_fin_big_split : forall {n} (v : t bool n),
     bitvector_fin_big v =
     exist (fun x => x < 2 ^ n)
-          (bitvector_fin_big_fun v)
-          (bitvector_fin_big_lim v).
+          (bitvector_nat_big v)
+          (bitvector_nat_big_lt_2pow v).
 Proof.
   intros n v.
   apply unique_fin; reflexivity.
@@ -333,24 +337,24 @@ Theorem bitvector_fin_big_inv : forall {n} (v : t bool n),
 Proof.
   intros n v.
   rewrite bitvector_fin_big_split.
-  simpl; rewrite bitvector_fin_big_fun_inv.
+  simpl; rewrite bitvector_nat_big_inv.
   reflexivity.
 Qed.
 
-Theorem fin_bitvector_big_fun_inv : forall n f,
+Theorem nat_bitvector_big_inv : forall n f,
   f < 2 ^ n ->
-  bitvector_fin_big_fun (fin_bitvector_big_fun n f) = f.
+  bitvector_nat_big (nat_bitvector_big n f) = f.
 Proof.
   intros n; induction n; intros f fP. 
-  - unfold bitvector_fin_big_fun.
+  - unfold bitvector_nat_big.
     simpl; simpl in fP; lia.
   - assert (2 ^ n <> 0) as pow0.
     { apply not_eq_sym, lt_neq, zero2pow. }
     assert ((f mod 2 ^ n) < 2 ^ n) as fl2n.
     { apply PeanoNat.Nat.mod_bound_pos; lia. }
-    simpl fin_bitvector_big_fun.
+    simpl nat_bitvector_big.
     destruct (f / 2 ^ n =? 0) eqn:fDiv0;
-    unfold bitvector_fin_big_fun;
+    unfold bitvector_nat_big;
     simpl bitvector_fin_big; unfold fin_cast, fin_max, fin_add;
     rewrite bitvector_fin_big_split; simpl;
     rewrite (IHn (f mod 2 ^ n) fl2n).
@@ -377,7 +381,7 @@ Proof.
   intros n [f fP].
   unfold fin_bitvector_big; rewrite bitvector_fin_big_split.
   apply subset_eq_compat.
-  rewrite (fin_bitvector_big_fun_inv n f); trivial.
+  rewrite (nat_bitvector_big_inv n f); trivial.
 Qed.
 
 (* Relating big to little endian *)
@@ -455,48 +459,122 @@ Proof.
   apply bitvector_fin_little_inv.
 Qed.
 
+(* Misc. Theorems *)
+
+Theorem bitvector_nat_big_app : 
+  forall {n m} (v1 : t bool n) (v2 : t bool m), 
+  bitvector_nat_big (v1 ++ v2) =
+  bitvector_nat_big v1 * 2 ^ m + bitvector_nat_big v2.
+Proof.
+  intros n m v1 v2; induction v1.
+  - reflexivity.
+  - simpl; repeat rewrite bitvector_nat_big_cons.
+    rewrite IHv1, PeanoNat.Nat.pow_add_r.
+    lia.
+Qed.
+
+Theorem bitvector_fin_big_0_0 : forall {n} (v : t bool n),
+  bv_eq v (Vector.const b0 n) =
+  (bitvector_nat_big v =? 0).
+Proof.
+  induction v.
+  - reflexivity.
+  - rewrite bitvector_nat_big_cons; simpl.
+    destruct h; simpl. 2: { apply IHv. }
+    symmetry; rewrite eqb_neq.
+    assert (0 < 2 ^ n). { apply zero2pow. } 
+    lia.
+Qed.
+
+Theorem bv_eq_equiv : forall {n} (v1 v2 : t bool n),
+  (bv_eq v1 v2 = true) <-> v1 = v2.
+Proof.
+  apply rect2.
+  - split; reflexivity.
+  - intros n v1 v2 IHv; split.
+    + simpl; intro H; apply andb_prop in H; destruct H.
+      rewrite iffb_beq in H; f_equal; auto.
+      rewrite <- IHv; assumption.
+    + intro H; injection H; intros veq eab.
+      apply inj_pair2 in veq.
+      simpl bv_eq; rewrite Bool.andb_true_iff; split.
+      * rewrite iffb_beq; assumption.
+      * rewrite IHv; assumption.
+Qed.
+
+Theorem bitvector_fin_big_0_const :
+  forall {n} (v : t bool n),
+    (v = (Vector.const b0 n)) <-> (bitvector_nat_big v = 0).
+Proof.
+  intros n v.
+  rewrite <- bv_eq_equiv, <- eqb_eq, <- Bool.eq_iff_eq_true.
+  apply bitvector_fin_big_0_0.
+Qed.
+
 (* Bitvector arithmetic *)
 
 (*least significant bits of addition (unsigned)
   extra leading bit indicates an overflow*)
 Definition bv_add {n} (b1 b2 : t bool n) : t bool (S n) :=
-  fin_bitvector_big_fun (S n)
-    (bitvector_fin_big_fun b1 + bitvector_fin_big_fun b2).
+  nat_bitvector_big (S n)
+    (bitvector_nat_big b1 + bitvector_nat_big b2).
 
-Theorem bv_add_correct : forall {n} (b1 b2 : t bool n),
-  bv_add b1 b2 = fin_bitvector_big_fun (S n)
-    (bitvector_fin_big_fun b1 + bitvector_fin_big_fun b2).
+Theorem bv_add_correct_1 : forall {n} (b1 b2 : t bool n),
+  bv_add b1 b2 = nat_bitvector_big (S n)
+    (bitvector_nat_big b1 + bitvector_nat_big b2).
 Proof. reflexivity. Qed.
 
+Theorem bv_add_correct_2 : forall {n} (n1 n2 : nat),
+  n1 < 2 ^ n -> n2 < 2 ^ n ->
+  n1 + n2 = bitvector_nat_big (
+  bv_add (nat_bitvector_big n n1) (nat_bitvector_big n n2)).
+Proof.
+  intros.
+  rewrite bv_add_correct_1.
+  repeat rewrite nat_bitvector_big_inv; try lia.
+  simpl; lia.
+Qed.
+
 Definition bv_incr {n} (i : nat) (v : t bool n) : t bool n :=
-  fin_bitvector_big_fun n ((i + bitvector_fin_big_fun v) mod (2 ^ n)).
+  nat_bitvector_big n ((i + bitvector_nat_big v) mod (2 ^ n)).
 
 (*least significant bits of subtraction (unsigned). 
   extra leading bit indicates a borrow, 0 if borrow, 1 if not.*)
 Definition bv_sub {n} (b1 b2 : t bool n) : t bool (S n) :=
-  fin_bitvector_big_fun (S n) 
-    (bitvector_fin_big_fun b1 + 2 ^ n - bitvector_fin_big_fun b2).
+  nat_bitvector_big (S n) 
+    (bitvector_nat_big b1 + 2 ^ n - bitvector_nat_big b2).
 
-Theorem bv_sub_correct : forall {n} (b1 b2 : t bool n),
-  bv_sub b1 b2 = fin_bitvector_big_fun (S n) 
-    (bitvector_fin_big_fun b1 + 2 ^ n - bitvector_fin_big_fun b2).
+Theorem bv_sub_correct_1 : forall {n} (b1 b2 : t bool n),
+  bv_sub b1 b2 = nat_bitvector_big (S n) 
+    (bitvector_nat_big b1 + 2 ^ n - bitvector_nat_big b2).
 Proof. reflexivity. Qed.
+
+Theorem bv_sub_correct_2 : forall {n} (n1 n2 : nat),
+  n1 < 2 ^ n -> n2 < 2 ^ n ->
+  n1 + 2 ^ n - n2 = bitvector_nat_big (
+  bv_sub (nat_bitvector_big n n1) (nat_bitvector_big n n2)).
+Proof. 
+  intros.
+  rewrite bv_sub_correct_1.
+  repeat rewrite nat_bitvector_big_inv; try lia.
+  simpl; lia.
+Qed.
 
 (*least significant bits of multiplication (unsigned)
   additional bits indicate, respecively, an overflow and a result of 0.
   Left vector are MSB, right vector are LSB.*)
 Definition bv_mul_flags {n} (b1 b2 : t bool n) : bool * bool * t bool n * t bool n :=
-  let prod := (bitvector_fin_big_fun b1 * bitvector_fin_big_fun b2) in
-  let (pvH, pvL) := splitat n (fin_bitvector_big_fun (n + n) prod) in
+  let prod := (bitvector_nat_big b1 * bitvector_nat_big b2) in
+  let (pvH, pvL) := splitat n (nat_bitvector_big (n + n) prod) in
   (2 ^ n <=? prod, prod =? 0, pvH, pvL).
 
 (*Multiplication (unsigned), all bits*)
 Definition bv_mul {n} (b1 b2 : t bool n) : t bool (n + n) :=
   (fun x => snd (fst x) ++ snd x) (bv_mul_flags b1 b2).
 
-Theorem bv_mul_correct : forall {n} (b1 b2 : t bool n),
-  bv_mul b1 b2 = fin_bitvector_big_fun (n + n) 
-    (bitvector_fin_big_fun b1 * bitvector_fin_big_fun b2).
+Theorem bv_mul_correct_1 : forall {n} (b1 b2 : t bool n),
+  bv_mul b1 b2 = nat_bitvector_big (n + n) 
+    (bitvector_nat_big b1 * bitvector_nat_big b2).
 Proof.
   intros n b2 b3.
   unfold bv_mul, bv_mul_flags.
@@ -505,38 +583,101 @@ Proof.
   symmetry; assumption.
 Qed.
 
+Theorem bv_mul_correct_2 : forall {n} (n1 n2 : nat),
+  n1 < 2 ^ n -> n2 < 2 ^ n ->
+  n1 * n2 = bitvector_nat_big (
+  bv_mul (nat_bitvector_big n n1) (nat_bitvector_big n n2)).
+Proof. 
+  intros.
+  rewrite bv_mul_correct_1.
+  repeat rewrite nat_bitvector_big_inv; try lia.
+  rewrite PeanoNat.Nat.pow_add_r.
+  apply PeanoNat.Nat.mul_lt_mono; lia.
+Qed.
+
+Theorem lt_mul_cap : 
+  forall a b c, 0 < c -> a + b * c < c -> b = 0.
+Proof.
+  intros.
+  assert (b * c < 1 * c) as bclt. { lia. }
+  rewrite <- PeanoNat.Nat.mul_lt_mono_pos_r in bclt; lia.
+Qed.
+
+Theorem bv_mull_high_const0 : forall {n} (b1 b2 : t bool n),
+  (bitvector_nat_big b1 * bitvector_nat_big b2 < 2 ^ n)
+  <-> (fst (splitat n (bv_mul b1 b2)) = const b0 _).
+Proof.
+  intros n b1 b2.
+  rewrite <- nat_bitvector_big_inv at 1.
+  2: { rewrite PeanoNat.Nat.pow_add_r.
+       apply PeanoNat.Nat.mul_lt_mono;
+       apply bitvector_nat_big_lt_2pow. }
+  rewrite <- bv_mul_correct_1.
+  destruct (splitat _ _) as [b12h b12l] eqn:sE; simpl fst.
+  apply Vector.append_splitat in sE; rewrite sE.
+  rewrite bitvector_nat_big_app.
+  split.
+  - intro; rewrite bitvector_fin_big_0_const.
+    rewrite add_comm in H. apply lt_mul_cap in H; lia.
+  - intro H; rewrite bitvector_fin_big_0_const in H.
+    rewrite H; simpl.
+    apply bitvector_nat_big_lt_2pow.
+Qed.
+
 (*unsigned division. Extra boolean indicates division by 0.*)
 Definition bv_udiv_flag {n} (b1 b2 : t bool n) : bool * t bool n :=
-  let den := bitvector_fin_big_fun b2 in
-  (den =? 0, fin_bitvector_big_fun n (bitvector_fin_big_fun b1 / den)).
+  let den := bitvector_nat_big b2 in
+  (den =? 0, nat_bitvector_big n (bitvector_nat_big b1 / den)).
 
 Definition bv_udiv {n} (b1 b2 : t bool n) : t bool n :=
   snd (bv_udiv_flag b1 b2).
 
-Theorem bv_udiv_correct : forall {n} (b1 b2 : t bool n),
-  bv_udiv b1 b2 = fin_bitvector_big_fun n 
-    (bitvector_fin_big_fun b1 / bitvector_fin_big_fun b2).
+Theorem bv_udiv_correct_1 : forall {n} (b1 b2 : t bool n),
+  bv_udiv b1 b2 = nat_bitvector_big n 
+    (bitvector_nat_big b1 / bitvector_nat_big b2).
 Proof.
   intros n b2 b3.
   unfold bv_udiv, bv_udiv_flag.
   reflexivity.
 Qed.
 
+Theorem bv_udiv_correct_2 : forall {n} (n1 n2 : nat),
+  n1 < 2 ^ n -> n2 < 2 ^ n -> n2 <> 0 ->
+  n1 / n2 = bitvector_nat_big (
+  bv_udiv (nat_bitvector_big n n1) (nat_bitvector_big n n2)).
+Proof. 
+  intros.
+  rewrite bv_udiv_correct_1.
+  repeat rewrite nat_bitvector_big_inv; try lia.
+  apply neq0_div_lt; assumption.
+Qed.
+
 (*unsigned modulus. Extra boolean indicates modulus by 0.*)
 Definition bv_umod_flag {n} (b1 b2 : t bool n) : bool * t bool n :=
-  let bas := bitvector_fin_big_fun b2 in
-  (bas =? 0, fin_bitvector_big_fun n (bitvector_fin_big_fun b1 mod bas)).
+  let bas := bitvector_nat_big b2 in
+  (bas =? 0, nat_bitvector_big n (bitvector_nat_big b1 mod bas)).
 
 Definition bv_umod {n} (b1 b2 : t bool n) : t bool n :=
   snd (bv_umod_flag b1 b2).
 
-Theorem bv_umod_correct : forall {n} (b1 b2 : t bool n),
-  bv_umod b1 b2 = fin_bitvector_big_fun n 
-    (bitvector_fin_big_fun b1 mod bitvector_fin_big_fun b2).
+Theorem bv_umod_correct_1 : forall {n} (b1 b2 : t bool n),
+  bv_umod b1 b2 = nat_bitvector_big n 
+    (bitvector_nat_big b1 mod bitvector_nat_big b2).
 Proof.
   intros n b2 b3.
   unfold bv_umod, bv_umod_flag.
   reflexivity.
+Qed.
+
+Theorem bv_umod_correct_2 : forall {n} (n1 n2 : nat),
+  n1 < 2 ^ n -> n2 < 2 ^ n -> n2 <> 0 ->
+  n1 mod n2 = bitvector_nat_big (
+  bv_umod (nat_bitvector_big n n1) (nat_bitvector_big n n2)).
+Proof. 
+  intros.
+  rewrite bv_umod_correct_1.
+  repeat rewrite nat_bitvector_big_inv; try lia.
+  rewrite PeanoNat.Nat.mod_eq; try lia.
 Qed.
 
 (*left-shift by m with zero padding.*)
@@ -611,12 +752,12 @@ Definition twos_complement {n} (v : t bool (S n)) : Z :=
   end.
 
 Theorem twos_complement_big : forall {n} (v : t bool n),
-  twos_complement' v = bitvector_fin_big_fun v.
+  twos_complement' v = bitvector_nat_big v.
 Proof.
   intros n v; induction v.
   - reflexivity.
   - simpl twos_complement'.
-    unfold bitvector_fin_big_fun.
+    unfold bitvector_nat_big.
     rewrite bitvector_fin_big_cons.
     rewrite proj1_fin_cast, proj1_fin_add, proj1_fin_mul,
             proj1_fin_max, proj1_bitVal.
@@ -655,13 +796,13 @@ Proof.
   rewrite Z_inj_pow.
   apply Znat.inj_lt.
   rewrite twos_complement_big.
-  apply bitvector_fin_big_fun_lt_2pow.
+  apply bitvector_nat_big_lt_2pow.
 Qed.
 
 Definition twos_complement_inv (n : nat) (z : Z) : t bool (S n) :=
   match ltb z 0 with
-  | true => fin_bitvector_big_fun _ (Z.to_nat (add z (pow 2 (of_nat (S n)))))
-  | false => fin_bitvector_big_fun _ (Z.to_nat z)
+  | true => nat_bitvector_big _ (Z.to_nat (add z (pow 2 (of_nat (S n)))))
+  | false => nat_bitvector_big _ (Z.to_nat z)
   end.
 
 Theorem twos_complement_iso_1 : forall {n} (v : t bool (S n)),
@@ -669,7 +810,7 @@ Theorem twos_complement_iso_1 : forall {n} (v : t bool (S n)),
 Proof.
   intros n v.
   assert (twos_complement' (tl v) < 2 ^ n).
-  { rewrite twos_complement_big; apply bitvector_fin_big_fun_lt_2pow. }
+  { rewrite twos_complement_big; apply bitvector_nat_big_lt_2pow. }
   rewrite (Vector.eta v).
   simpl.
   destruct (hd v); simpl bitValN.
@@ -687,31 +828,31 @@ Proof.
     replace (2 ^ S n - 2 ^ n) with (2 ^ n). 2: { simpl; lia. }
     rewrite BinInt.Z.sub_opp_r, <- Znat.Nat2Z.inj_add.
     rewrite Znat.Nat2Z.id.
-    unfold fin_bitvector_big_fun; f_equal.
+    unfold nat_bitvector_big; f_equal.
     + replace (_ / _) with 1. { reflexivity. }
       symmetry; apply div_bet_1; lia.
-    + fold fin_bitvector_big_fun.
+    + fold nat_bitvector_big.
       assert (2 ^ n <> 0).
       { apply PeanoNat.Nat.pow_nonzero; lia. }
       rewrite <- PeanoNat.Nat.add_mod_idemp_r. 2: { assumption. }
       rewrite PeanoNat.Nat.mod_same. 2: { assumption. }
       rewrite add_0_r, mod_small. 2: { assumption. }
       rewrite twos_complement_big. 
-      apply bitvector_fin_big_fun_inv.
+      apply bitvector_nat_big_inv.
   - simpl of_nat; rewrite BinInt.Z.sub_0_r.
     unfold twos_complement_inv.
     replace (ltb (of_nat (twos_complement' (tl v))) 0)
        with false.
     2: { symmetry; rewrite Z_nltb_ge. apply Znat.Nat2Z.is_nonneg. }
     rewrite Znat.Nat2Z.id.
-    unfold fin_bitvector_big_fun; fold fin_bitvector_big_fun.
+    unfold nat_bitvector_big; fold nat_bitvector_big.
     f_equal.
     + replace (_ / _) with 0. { reflexivity. }
       symmetry; apply div_small; assumption.
     + replace (_ mod _) with (twos_complement' (tl v)).
       2: { symmetry; apply mod_small; assumption. }
       rewrite twos_complement_big.
-      apply bitvector_fin_big_fun_inv.
+      apply bitvector_nat_big_inv.
 Qed.
 
 Theorem twos_complement_iso_2 : forall n z,
@@ -731,8 +872,8 @@ Proof.
     rewrite Z2_inj_pow; try lia.
     change (to_nat _) with 2 at 1.
     rewrite Znat.Nat2Z.id.
-    unfold fin_bitvector_big_fun, twos_complement;
-    fold fin_bitvector_big_fun.
+    unfold nat_bitvector_big, twos_complement;
+    fold nat_bitvector_big.
     assert ((to_nat (opp z)) <= 2 ^ n).
     { rewrite <- Znat.Nat2Z.id, <- Znat.Z2Nat.inj_le; try lia;
       rewrite opp_le_swap_l, <- Z_inj_pow; exact lez. }
@@ -743,15 +884,15 @@ Proof.
          rewrite <- PeanoNat.Nat.add_mod_idemp_l, PeanoNat.Nat.mod_same.
          simpl. symmetry; apply mod_small; lia. assumption. assumption.
          simpl; lia. }
-    simpl; rewrite twos_complement_big, fin_bitvector_big_fun_inv; lia.
+    simpl; rewrite twos_complement_big, nat_bitvector_big_inv; lia.
   - rewrite Z_nltb_ge in ltz0.
     assert (0 <= to_nat z). { lia. }
     assert (to_nat z < 2 ^ n).
     { rewrite Znat.Z2Nat.inj_lt, Z2_inj_pow, Znat.Nat2Z.id in ltz; try lia.
       assumption. }
-    unfold fin_bitvector_big_fun; fold fin_bitvector_big_fun.
+    unfold nat_bitvector_big; fold nat_bitvector_big.
     rewrite mod_small, div_small; try assumption.
-    simpl; rewrite twos_complement_big, fin_bitvector_big_fun_inv; lia.
+    simpl; rewrite twos_complement_big, nat_bitvector_big_inv; lia.
 Qed.
 
 Theorem twos_complement_sign : forall n z,
@@ -761,7 +902,7 @@ Theorem twos_complement_sign : forall n z,
 Proof.
   intros n z zmin zmax.
   unfold twos_complement_inv.
-  destruct (ltb z 0) eqn:ltz0; unfold fin_bitvector_big_fun.
+  destruct (ltb z 0) eqn:ltz0; unfold nat_bitvector_big.
   - rewrite Z_ltb_lt in ltz0.
     replace (_ / _) with 1. { reflexivity. }
     rewrite BinInt.Z.add_comm, <- BinInt.Z.sub_opp_r.
@@ -785,7 +926,7 @@ Qed.
 
 (*Absolute value of signed vector*)
 Definition bv_abs {n} (v : t bool (S n)) : t bool n :=
-  fin_bitvector_big_fun n (Z.abs_nat (twos_complement v)).
+  nat_bitvector_big n (Z.abs_nat (twos_complement v)).
 (*
 Definition bv_abs {n} (v : t bool (S n)) : t bool n :=
   match v with
@@ -798,7 +939,7 @@ Definition bv_abs {n} (v : t bool (S n)) : t bool n :=
 *)
 
 Theorem bv_abs_correct : forall {n} (v : t bool (S n)),
-  bv_abs v = fin_bitvector_big_fun n (Z.abs_nat (twos_complement v)).
+  bv_abs v = nat_bitvector_big n (Z.abs_nat (twos_complement v)).
 Proof. reflexivity. Qed.
 
 (*Negative of signed vector*)
@@ -851,6 +992,38 @@ Proof.
   - apply lt_mul_mul; lia.
 Qed.
 
+Theorem bv_smul_correct_sign : forall {n} (b1 b2 : t bool (S n)),
+  (lt (opp (pow 2 (of_nat n))) (twos_complement b1)) ->
+  (lt (opp (pow 2 (of_nat n))) (twos_complement b2))->
+  hd (bv_smul b1 b2) = ltb (mul (twos_complement b1) (twos_complement b2)) 0.
+Proof.
+  intros n b1 b2.
+  rewrite bv_smul_correct_1.
+  intros min1 min2.
+  remember (mul _ _) as m.
+  unfold twos_complement_inv.
+  destruct (ltb _ _) eqn:ltm.
+  - change 2%Z with (of_nat 2).
+    unfold nat_bitvector_big; change (hd (?x :: _)) with x.
+    rewrite Z_inj_pow, <- (BinInt.Z.opp_involutive m), BinInt.Z.add_opp_l,
+            Znat.Z2Nat.inj_sub, Znat.Nat2Z.id; try lia.
+    replace (_ / _) with 1. { reflexivity. }
+    assert (to_nat (opp m) <= 2 ^ (n + n)).
+    { rewrite <- Znat.Nat2Z.id, <- Znat.Z2Nat.inj_le; try lia.
+      rewrite <- Z_inj_pow, Znat.Nat2Z.inj_add, BinInt.Z.pow_add_r; try lia.
+      rewrite <- BinInt.Z.pow_add_r, Heqm, opp_le_swap_l, BinInt.Z.pow_add_r; try lia.
+      apply le_opp_mul_mul; try lia; apply twos_complement_max. }
+    symmetry; apply div_bet_1; split; simpl; lia.
+  - rewrite BinInt.Z.ltb_ge in ltm.
+    unfold nat_bitvector_big; change (hd (?x :: _)) with x.
+    replace (_ / _) with 0. { reflexivity. }
+    symmetry; apply div_small.
+    rewrite <- Znat.Nat2Z.id, <- Znat.Z2Nat.inj_lt; try lia.
+    rewrite <- Z_inj_pow, Znat.Nat2Z.inj_add, BinInt.Z.pow_add_r; try lia.
+    rewrite <- BinInt.Z.pow_add_r, Heqm, BinInt.Z.pow_add_r; try lia.
+    apply lt_mul_mul; try lia; apply twos_complement_max.
+Qed.
+
 (* Computes the upper n bits of the signed multiplication
    of two two's-complement numbers.
 
@@ -869,13 +1042,13 @@ Definition bv_smulh : forall {n} (b1 b2 : t bool (S n)),
   apply cons.
   - exact (ltb b12 Z0).
   - apply (fun (x : t bool (n + n)) => fst (splitat n x)), 
-          fin_bitvector_big_fun, Z.abs_nat, b12.
+          nat_bitvector_big, Z.abs_nat, b12.
 Defined.
 
 Theorem bv_smulh_correct_value :
   forall {n} (b1 b2 : t bool (S n)), 
   tl (bv_smulh b1 b2) = 
-    fst (splitat n (fin_bitvector_big_fun (n + n) 
+    fst (splitat n (nat_bitvector_big (n + n) 
     (Z.abs_nat (mul (twos_complement b1) (twos_complement b2))))).
 Proof. reflexivity. Qed.
 
